Introduce preliminary bignum/nat conversion

code/experimental/rsapss/Hacl.Impl.Bignum.Convert.fst
@@ -12,12 +12,14 @@ open Lib.ByteBuffer
 
 open Hacl.Impl.Bignum.Core
 
+module Seq = Lib.Sequence
+module B = FStar.Bytes
 module ST = FStar.HyperStack.ST
 
-#reset-options "--z3rlimit 100 --max_fuel 0 --max_ifuel 0"
+#reset-options "--z3rlimit 150 --max_fuel 0 --max_ifuel 0"
 
 inline_for_extraction noextract
-val text_to_nat_:
+val bytes_to_bignum_:
     len:size_t
   -> input:lbuffer8 len
   -> resLen:size_t{v len = 8 * v resLen}
@@ -25,7 +27,7 @@ val text_to_nat_:
   -> Stack unit
     (requires fun h -> live h input /\ live h res /\ disjoint res input)
     (ensures  fun h0 _ h1 -> modifies (loc res) h0 h1)
-let text_to_nat_ len input resLen res =
+let bytes_to_bignum_ len input resLen res =
   let h0 = ST.get () in
   let inv h1 i = modifies (loc res) h0 h1 in
   Lib.Loops.for 0ul resLen inv
@@ -33,7 +35,7 @@ let text_to_nat_ len input resLen res =
     res.(resLen -. i -. 1ul) <- uint_from_bytes_be (sub input (8ul *. i) 8ul)
   )
 
-val text_to_nat:
+val bytes_to_bignum:
     len:size_t{v len > 0}
   -> input:lbuffer8 len
   -> res:lbignum (blocks len 8ul){8 * v (blocks len 8ul) < max_size_t}
@@ -41,7 +43,7 @@ val text_to_nat:
     (requires fun h -> live h input /\ live h res /\ disjoint res input)
     (ensures  fun h0 _ h1 -> modifies (loc res) h0 h1)
 [@"c_inline"]
-let text_to_nat len input res =
+let bytes_to_bignum len input res =
   push_frame ();
   let num_words = blocks len 8ul in
   let tmpLen = 8ul *. num_words in
@@ -52,11 +54,11 @@ let text_to_nat len input res =
   let tmpLen1 = tmpLen -. ind in
   let tmp1 = sub tmp ind tmpLen1 in
   copy tmp1 input;
-  text_to_nat_ tmpLen tmp num_words res;
+  bytes_to_bignum_ tmpLen tmp num_words res;
   pop_frame ()
 
 inline_for_extraction noextract
-val nat_to_text_:
+val bignum_to_bytes_:
     len:size_t
   -> input:lbignum len
   -> resLen:size_t{v resLen = 8 * v len}
@@ -64,7 +66,7 @@ val nat_to_text_:
   -> Stack unit
     (requires fun h -> live h input /\ live h res /\ disjoint res input)
     (ensures  fun h0 _ h1 -> modifies (loc res) h0 h1)
-let nat_to_text_ len input resLen res =
+let bignum_to_bytes_ len input resLen res =
   let h0 = ST.get () in
   let inv h1 i = modifies (loc res) h0 h1 in
   Lib.Loops.for 0ul len inv
@@ -73,7 +75,7 @@ let nat_to_text_ len input resLen res =
     uint_to_bytes_be (sub res (8ul *. i) 8ul) tmp
   )
 
-val nat_to_text:
+val bignum_to_bytes:
     len:size_t{v len > 0}
   -> input:lbignum (blocks len 8ul){8 * v (blocks len 8ul) < max_size_t}
   -> res:lbuffer8 len
@@ -81,7 +83,7 @@ val nat_to_text:
     (requires fun h -> live h input /\ live h res /\ disjoint res input)
     (ensures  fun h0 _ h1 -> modifies (loc res) h0 h1)
 [@"c_inline"]
-let nat_to_text len input res = admit();
+let bignum_to_bytes len input res = admit();
   push_frame ();
   let num_words = blocks len 8ul in
   let tmpLen = 8ul *. num_words in
@@ -89,8 +91,75 @@ let nat_to_text len input res = admit();
   let ind = if m =. 0ul then 0ul else 8ul -. m in
 
   let tmp = create tmpLen (u8 0) in
-  nat_to_text_ num_words input tmpLen tmp;
+  bignum_to_bytes_ num_words input tmpLen tmp;
   let tmpLen1 = tmpLen -. ind in
   let tmp1 = sub tmp ind tmpLen1 in
   copy res tmp1;
   pop_frame ()
+
+// This version does not work, because of the internal rec I think.
+//
+//inline_for_extraction noextract
+//val nat_to_list64: nat -> list pub_uint64
+//let nat_to_list64 x =
+//  [@inline_let]
+//  let rec go (y: nat) =
+//    if y <= maxint U64
+//    then [uint y]
+//    else uint (y % 64) :: go (y / 64)kin
+//  go x
+
+
+inline_for_extraction noextract
+val nat_to_list64: nat -> list pub_uint64
+let rec nat_to_list64 y = admit();
+    if y <= maxint U64
+    then [uint y]
+    else uint (y % 64) :: nat_to_list64 (y / 64)
+
+inline_for_extraction noextract
+val nat_to_list64_sec: nat -> list uint64
+let nat_to_list64_sec x = List.Tot.map secret (nat_to_list64 x)
+
+inline_for_extraction noextract
+val nat_bytes_num: nat -> size_t
+let nat_bytes_num x = admit(); normalize_term (size (List.Tot.length (nat_to_list64_sec x)))
+
+
+inline_for_extraction noextract
+val nat_to_bignum_exact:
+     input:nat
+  -> StackInline (lbignum (nat_bytes_num input))
+    (requires fun _ -> true)
+    (ensures  fun h0 b h1 -> modifies (loc b) h0 h1)
+let nat_to_bignum_exact input =
+  [@inline_let]
+  let l: list uint64 = normalize_term (nat_to_list64_sec input) in
+  assume (List.Tot.length l <= max_size_t);
+  assume (normalize (List.Tot.length l <= max_size_t));
+  [@inline_let]
+  let len: size_t = nat_bytes_num input in
+  admit();
+  createL l
+
+
+inline_for_extraction noextract
+val nat_to_bignum:
+     #k:size_t{v k > 0}
+  -> input:nat { v (nat_bytes_num input) <= v k }
+  -> StackInline (lbignum k)
+    (requires fun _ -> true)
+    (ensures  fun h0 b h1 -> modifies (loc b) h0 h1)
+let nat_to_bignum #k input =
+  admit();
+  push_frame ();
+
+  let len: size_t = nat_bytes_num input in
+  let created: lbignum len = nat_to_bignum_exact input in
+  let res: lbignum k = create k (u64 0) in
+  let res_sub: lbignum len = sub res 0ul len in
+
+  let h0 = ST.get () in
+  copy res_sub created;
+  pop_frame ();
+  res
