code/experimental/rsapss/Hacl.Test.RSA.fst
@@ -70,17 +70,17 @@ let ctest pow2_i modBits n pkeyBits e skeyBits d pTLen p qTLen q r2 rBlindTLen r
   let qNat = sub skey (pkeyLen +. dLen +. pLen) qLen in
 
 
-  text_to_nat (blocks modBits 8ul) n nNat;
-  text_to_nat (blocks pkeyBits 8ul) e eNat;
-  text_to_nat (blocks modBits 8ul) r2 r2Nat;
-  text_to_nat (blocks skeyBits 8ul) d dNat;
-  text_to_nat pTLen p pNat;
-  text_to_nat qTLen q qNat;
+  bytes_to_bignum (blocks modBits 8ul) n nNat;
+  bytes_to_bignum (blocks pkeyBits 8ul) e eNat;
+  bytes_to_bignum (blocks modBits 8ul) r2 r2Nat;
+  bytes_to_bignum (blocks skeyBits 8ul) d dNat;
+  bytes_to_bignum pTLen p pNat;
+  bytes_to_bignum qTLen q qNat;
 
   let pkey = sub skey 0ul pkeyLen in
 
   let rBlindNat = create rBlindLen (u64 0) in
-  text_to_nat rBlindTLen rBlind rBlindNat;
+  bytes_to_bignum rBlindTLen rBlind rBlindNat;
   let rBlind0 = rBlindNat.(0ul) in
 
   let nTLen = blocks modBits 8ul in
